[tactics] Remove unused definitions.

theories/proofmode/tactics.v
@@ -11,135 +11,24 @@ From osiris.semantics Require Import semantics.
 From osiris.weakestpre Require Import weakestpre.
 From osiris.proofmode Require Import simp.
 
-(* -------------------------------------------------------------------------- *)
+(* ---------------------------------------------------------------------- *)
+(* Tactics to work on WPs. They mimic those on [is_safe]. *)
 
-(* Auxiliary definitions *)
+Lemma tac_change_goal {Σ: gFunctors} Δ (P Q : iProp Σ) :
+  (P ⊢ Q) →
+  environments.envs_entails Δ P →
+  environments.envs_entails Δ Q.
+Proof.
+  intros H Henv.
+  eapply coq_tactics.tac_eval; last done.
+  intros Q''; subst Q''. assumption.
+Qed.
 
-Fixpoint environment_support η : list string :=
-  match η with
-  | EnvNil => []
-  | EnvCons s _ η => s :: environment_support η
-  end.
-
-Definition spec_support `{!osirisGS_gen hlc Σ} : list (string * (val → iProp Σ)) → list string :=
-  List.map fst.
-
-Fixpoint in_bool' (s : string) (l : list string) : bool * list string :=
-  match l with
-  | [] => (false, [])
-  | h :: l =>
-      if (s =? h)%string
-      then (true, l)
-      else match in_bool' s l with
-           | (true, l) => (true, h :: l)
-           | (false, _) => (false, h :: l)
-           end
-  end.
-
-Fixpoint in_bool (s : string) (l : list string) : bool :=
-  match l with
-  | [] => false
-  | h :: l =>
-      if (s =? h)%string
-      then true
-      else in_bool s l
-  end.
-
-Global Instance string_list_intersection : Intersection (list string) :=
-  fix go l l' :=
-    match l with
-    | [] => []
-    | h :: l =>
-        match in_bool' h l' with
-        | (false, l') => go l l'
-        | (true, l') => h :: go l l'
-        end
-    end.
-
-Global Instance string_list_difference : Difference (list string) :=
-  fix go l l' :=
-    match l with
-    | [] => []
-    | h :: l =>
-        match in_bool h l' with
-        | false => h :: go l l'
-        | true => go l l'
-        end
-    end.
-
-Definition has_specs `{!osirisGS_gen hlc Σ} (η: env) (Λ: list (string * (val → iProp Σ))) :=
-  match intersection (environment_support η)
-                     (spec_support Λ) with
-  | [] => false
-  | _ => true
-  end.
-
-Fixpoint from_pattern (p: pat) : list string :=
-  match p with
-  | PAny => []
-  | PVar v => [v]
-  | PAlias p v => v :: from_pattern p
-  | PTuple ps => from_patterns ps
-  | POr p1 p2 => (* Over approximation. *)
-      from_pattern p1 ++ from_pattern p2
-  | PData _ p => from_pattern p
-  | PRecord fps => from_fpatterns fps
-  | _ => [] (* Constants. *)
-  end
-with from_fpatterns fps :=
-       match fps with
-       | FPNil => []
-       | FPCons _ p fps => from_pattern p ++ from_fpatterns fps
-       end
-with from_patterns (ps: pats) : list string :=
-       match ps with
-       | PNil => []
-       | PCons p ps => from_pattern p ++ from_patterns ps
-       end.
-
-Definition module_defines (m: mexpr) : list string :=
-  let from_bindings : bindings → list string :=
-    fix go bds :=
-      match bds with
-      | BiNil => []
-      | BiCons (Binding p _) bds =>
-          from_pattern p ++ go bds
-      end
-  in
-  let from_rec_bindings : rec_bindings → list string :=
-    fix go bds :=
-      match bds with
-      | RecBiNil => []
-      | RecBiCons (RecBinding v _) bds =>
-          v :: go bds
-      end
-  in
-  let from_item : sitem → list string :=
-    fun item =>
-      match item with
-      | ILet bds => from_bindings bds
-      | ILetRec bds => from_rec_bindings bds
-      | _ => [] (* TODO. *)
-      end
-  in
-  let from_items : sitems → list string :=
-    fix go items :=
-      match items with
-      | INil => []
-      | ICons item items =>
-          from_item item ++ go items
-      end
-  in
-  match m with
-  | MStruct items => from_items items
-  | _ => [] (* TODO. *)
-  end.
-
-Definition id_spec {A} (a: A) := a.
-Global Opaque id_spec.
-
-Definition id_continue {A} (a: A) := a.
-Global Opaque id_continue.
+(* [lem] must be of the form (P -∗ Q). Thanks to the tactic notation it can be
+   lemma whose forall quantifiers have been instantiated with [_]. *)
+Ltac tac_change_goal lem :=
+  simple notypeclasses refine (tac_change_goal _ _ _ lem _).
+Tactic Notation "tac_change_goal" uconstr(lem) := (tac_change_goal lem).
 
 (* -------------------------------------------------------------------------- *)
 
@@ -229,29 +118,7 @@ Ltac wp_concat :=
   end.
 
 Local Ltac wp_startproof :=
-  iStartProof;
-  lazymatch goal with
-  | _ := id_continue _ |- _=> idtac
-  | |- environments.envs_entails _ $ wp _ _ (eval_mexpr _ ?m) (module_spec ?Λ) =>
-      let from_module := eval cbn in (module_defines m) in
-      let from_spec := eval cbn in (List.map fst Λ) in
-      let diff := eval cbn in (difference from_module from_spec) in
-      pose (__osiris_continue := id_continue diff);
-      pose (__osiris_specs := id_spec Λ)
-  | |- _ => idtac
-  end.
-
-Local Ltac wp_continue_if_nospec :=
-  lazymatch goal with
-  | _ := id_continue ?l |- environments.envs_entails _ $ wp _ _ (ret_dconcat ?δ _) _ =>
-    let δ := eval cbn in (environment_support δ) in
-    let ret := eval cbn in (forallb (fun s => in_bool s l) δ) in
-      lazymatch constr:(ret) with
-      | true => wp_concat
-      | false => idtac
-      end
-  | _ => fail "Cannot continue."
-  end.
+  iStartProof.
 
 Ltac wp :=
   wp_startproof;
@@ -267,9 +134,6 @@ Ltac wp :=
           progress wp_simp
         | (* 3. *)
           progress cbn
-        | (* 4. Experimental: try to automatically mimic [wp_continue]
-                sometimes. *)
-          wp_continue_if_nospec
         | (* Otherwise, do nothing ([repeat] will stop). *)
           idtac
     ]);
