attic/proofmode_tactics.v
@@ -1,0 +1,131 @@
+
+(* -------------------------------------------------------------------------- *)
+
+(* Auxiliary definitions *)
+
+Fixpoint environment_support η : list string :=
+  match η with
+  | EnvNil => []
+  | EnvCons s _ η => s :: environment_support η
+  end.
+
+Definition spec_support `{!osirisGS_gen hlc Σ} : list (string * (val → iProp Σ)) → list string :=
+  List.map fst.
+
+Fixpoint in_bool' (s : string) (l : list string) : bool * list string :=
+  match l with
+  | [] => (false, [])
+  | h :: l =>
+      if (s =? h)%string
+      then (true, l)
+      else match in_bool' s l with
+           | (true, l) => (true, h :: l)
+           | (false, _) => (false, h :: l)
+           end
+  end.
+
+Fixpoint in_bool (s : string) (l : list string) : bool :=
+  match l with
+  | [] => false
+  | h :: l =>
+      if (s =? h)%string
+      then true
+      else in_bool s l
+  end.
+
+Global Instance string_list_intersection : Intersection (list string) :=
+  fix go l l' :=
+    match l with
+    | [] => []
+    | h :: l =>
+        match in_bool' h l' with
+        | (false, l') => go l l'
+        | (true, l') => h :: go l l'
+        end
+    end.
+
+Global Instance string_list_difference : Difference (list string) :=
+  fix go l l' :=
+    match l with
+    | [] => []
+    | h :: l =>
+        match in_bool h l' with
+        | false => h :: go l l'
+        | true => go l l'
+        end
+    end.
+
+Definition has_specs `{!osirisGS_gen hlc Σ} (η: env) (Λ: list (string * (val → iProp Σ))) :=
+  match intersection (environment_support η)
+                     (spec_support Λ) with
+  | [] => false
+  | _ => true
+  end.
+
+Fixpoint from_pattern (p: pat) : list string :=
+  match p with
+  | PAny => []
+  | PVar v => [v]
+  | PAlias p v => v :: from_pattern p
+  | PTuple ps => from_patterns ps
+  | POr p1 p2 => (* Over approximation. *)
+      from_pattern p1 ++ from_pattern p2
+  | PData _ p => from_pattern p
+  | PRecord fps => from_fpatterns fps
+  | _ => [] (* Constants. *)
+  end
+with from_fpatterns fps :=
+       match fps with
+       | FPNil => []
+       | FPCons _ p fps => from_pattern p ++ from_fpatterns fps
+       end
+with from_patterns (ps: pats) : list string :=
+       match ps with
+       | PNil => []
+       | PCons p ps => from_pattern p ++ from_patterns ps
+       end.
+
+Definition module_defines (m: mexpr) : list string :=
+  let from_bindings : bindings → list string :=
+    fix go bds :=
+      match bds with
+      | BiNil => []
+      | BiCons (Binding p _) bds =>
+          from_pattern p ++ go bds
+      end
+  in
+  let from_rec_bindings : rec_bindings → list string :=
+    fix go bds :=
+      match bds with
+      | RecBiNil => []
+      | RecBiCons (RecBinding v _) bds =>
+          v :: go bds
+      end
+  in
+  let from_item : sitem → list string :=
+    fun item =>
+      match item with
+      | ILet bds => from_bindings bds
+      | ILetRec bds => from_rec_bindings bds
+      | _ => [] (* TODO. *)
+      end
+  in
+  let from_items : sitems → list string :=
+    fix go items :=
+      match items with
+      | INil => []
+      | ICons item items =>
+          from_item item ++ go items
+      end
+  in
+  match m with
+  | MStruct items => from_items items
+  | _ => [] (* TODO. *)
+  end.
+
+Definition id_spec {A} (a: A) := a.
+Global Opaque id_spec.
+
+Definition id_continue {A} (a: A) := a.
+Global Opaque id_continue.
+
