theories/weakestpre/weakestpre.v
@@ -2,6 +2,5 @@
 
 From osiris.weakestpre Require Export
      wp
-     wp_tactics
      specifications
 .
